GateRules.v
@@ -1,0 +1,59 @@
+Require Import externals.QuantumLib.Quantum.
+Require Export ZX.
+Require Export Gates.
+Require Export Rules.
+
+
+Lemma ZX_H_is_H : ZX_semantics ZX_H = Cexp (PI/4)%R .* hadamard.
+Proof.
+  simpl.
+  unfold Spider_Semantics_Impl, bra_ket_MN.
+  solve_matrix; 
+  field_simplify_eq [Cexp_PI2 Cexp_PI4 Ci2 Csqrt2_sqrt2_inv Csqrt2_inv]; 
+  try apply c_proj_eq; try simpl; try R_field_simplify; try reflexivity; (try split; try apply RtoC_neq; try apply sqrt2_neq_0; try auto).
+Qed.
+
+Lemma ZX_H_H_is_Wire : ZX_semantics (Compose ZX_H ZX_H) = Cexp (PI/2)%R .* ZX_semantics Wire.
+Proof.
+  Opaque ZX_H.
+  simpl.
+  Transparent ZX_H.
+  rewrite wire_identity_semantics.
+  rewrite ZX_H_is_H.
+  rewrite Mscale_mult_dist_l.
+  rewrite Mscale_mult_dist_r.
+  rewrite MmultHH.
+  rewrite Mscale_assoc.
+  rewrite <- Cexp_add.
+  assert ((PI/4+PI/4 = PI/2)%R) as H by lra.
+  rewrite H.
+  reflexivity.
+Qed.
+
+
+Local Open Scope R_scope.
+Lemma ZX_CNOT_l_is_cnot : ZX_semantics ZX_CNOT_l = (/ √ 2)%C .* cnot.
+Proof.
+  simpl.
+  unfold Spider_Semantics_Impl, bra_ket_MN.
+  rewrite wire_identity_semantics.
+  rewrite Cexp_0.
+  solve_matrix.
+Qed.
+
+Lemma ZX_CNOT_r_is_cnot : ZX_semantics ZX_CNOT_r = (/ √ 2)%C .* cnot.
+Proof.
+  simpl.
+  unfold Spider_Semantics_Impl, bra_ket_MN.
+  rewrite wire_identity_semantics.
+  rewrite Cexp_0.
+  solve_matrix.
+Qed.
+
+Lemma ZX_CNOT_equiv : ZX_semantics ZX_CNOT_l = ZX_semantics ZX_CNOT_r.
+Proof.
+  rewrite ZX_CNOT_l_is_cnot.
+  rewrite <- ZX_CNOT_r_is_cnot.
+Qed.
+
+Local Close Scope R_scope.
