Gates.v
@@ -1,0 +1,29 @@
+Require Import externals.QuantumLib.Quantum.
+Require Export ZX.
+
+Definition ZX_H := 
+    (Compose 
+        (@Z_Spider 1 1 (PI/2)) 
+        (Compose 
+            (@X_Spider 1 1(PI/2)) 
+            (@Z_Spider 1 1 (PI/2)))).
+
+Definition ZX_CNOT_l : ZX 2 2 := 
+    (Compose 
+        (Stack 
+            (@Z_Spider 1 2 0%R) 
+            Wire) 
+        (Stack 
+            Wire 
+            (@X_Spider 2 1 0%R))).
+
+Definition ZX_CNOT_r : ZX 2 2 := 
+    (Compose 
+        (Stack 
+            Wire 
+            (@X_Spider 1 2 0%R))
+        (Stack 
+            (@Z_Spider 2 1 0%R) 
+            Wire)).
+
+Notation ZX_CNOT := ZX_CNOT_l.
