Rules.v
@@ -1,0 +1,23 @@
+Require Import externals.QuantumLib.Quantum.
+Require Export ZX.
+
+Lemma Z_0_eq_X_0 : ZX_semantics (@Z_Spider 1 1 0) = ZX_semantics (@X_Spider 1 1 0).
+Proof.
+  simpl.
+  unfold Spider_Semantics_Impl; unfold bra_ket_MN.
+  unfold kron_n.
+  repeat rewrite kron_1_l; try auto with wf_db.
+  rewrite Cexp_0.
+  solve_matrix.
+Qed.
+
+Theorem identity_removal_Z : ZX_semantics (@Z_Spider 1 1 0) = ZX_semantics Wire.
+Proof.
+  reflexivity.
+Qed.
+
+Theorem identity_removal_X : ZX_semantics (@X_Spider 1 1 0) = ZX_semantics Wire.
+Proof.
+  rewrite <- Z_0_eq_X_0.
+  reflexivity.
+Qed.
